<?xml version="1.0"?>
<rdf:RDF xmlns="http://www.semanticweb.org/user/ontologies/2020/CovidOntology/1.0.0#"
     xml:base="http://www.semanticweb.org/user/ontologies/2020/CovidOntology/1.0.0"
     xmlns:owl="http://www.w3.org/2002/07/owl#"
     xmlns:rdf="http://www.w3.org/1999/02/22-rdf-syntax-ns#"
     xmlns:xml="http://www.w3.org/XML/1998/namespace"
     xmlns:xsd="http://www.w3.org/2001/XMLSchema#"
     xmlns:rdfs="http://www.w3.org/2000/01/rdf-schema#"
     xmlns:CovidOntology="http://www.semanticweb.org/user/ontologies/2020/CovidOntology/1.0.0#">
    <owl:Ontology rdf:about="http://www.semanticweb.org/user/ontologies/2020/CovidOntology/1.0.0"/>
    


    <!-- 
    ///////////////////////////////////////////////////////////////////////////////////////
    //
    // Object Properties
    //
    ///////////////////////////////////////////////////////////////////////////////////////
     -->

    


    <!-- http://www.semanticweb.org/user/ontologies/2020/CovidOntology/1.0.0#hasCase -->

    <owl:ObjectProperty rdf:about="http://www.semanticweb.org/user/ontologies/2020/CovidOntology/1.0.0#hasCase">
        <rdfs:subPropertyOf rdf:resource="http://www.w3.org/2002/07/owl#topObjectProperty"/>
        <rdfs:range rdf:resource="http://www.semanticweb.org/user/ontologies/2020/CovidOntology/1.0.0#Case"/>
        <owl:propertyDisjointWith rdf:resource="http://www.semanticweb.org/user/ontologies/2020/CovidOntology/1.0.0#hasDay"/>
        <owl:propertyDisjointWith rdf:resource="http://www.semanticweb.org/user/ontologies/2020/CovidOntology/1.0.0#hasRegion"/>
        <rdfs:comment>This is not a specific instance of covid. It is a set of known covid occurences in a given time and place.</rdfs:comment>
    </owl:ObjectProperty>
    


    <!-- http://www.semanticweb.org/user/ontologies/2020/CovidOntology/1.0.0#hasCountry -->

    <owl:ObjectProperty rdf:about="http://www.semanticweb.org/user/ontologies/2020/CovidOntology/1.0.0#hasCountry">
        <rdfs:subPropertyOf rdf:resource="http://www.w3.org/2002/07/owl#topObjectProperty"/>
        <rdfs:domain rdf:resource="http://www.semanticweb.org/user/ontologies/2020/CovidOntology/1.0.0#Region"/>
        <rdfs:range rdf:resource="http://www.semanticweb.org/user/ontologies/2020/CovidOntology/1.0.0#Country"/>
        <rdfs:comment>This property entails what country a Region is within.
It is not an inverse of hasRegion since both Countries and Cases have regions.</rdfs:comment>
    </owl:ObjectProperty>
    


    <!-- http://www.semanticweb.org/user/ontologies/2020/CovidOntology/1.0.0#hasDay -->

    <owl:ObjectProperty rdf:about="http://www.semanticweb.org/user/ontologies/2020/CovidOntology/1.0.0#hasDay">
        <rdfs:subPropertyOf rdf:resource="http://www.w3.org/2002/07/owl#topObjectProperty"/>
        <rdfs:domain rdf:resource="http://www.semanticweb.org/user/ontologies/2020/CovidOntology/1.0.0#Case"/>
        <rdfs:range rdf:resource="http://www.semanticweb.org/user/ontologies/2020/CovidOntology/1.0.0#Day"/>
        <rdfs:comment>This is the Day entity in which the case of covid occured.
Allows for quick reference to other cases during a given day.</rdfs:comment>
    </owl:ObjectProperty>
    


    <!-- http://www.semanticweb.org/user/ontologies/2020/CovidOntology/1.0.0#hasRegion -->

    <owl:ObjectProperty rdf:about="http://www.semanticweb.org/user/ontologies/2020/CovidOntology/1.0.0#hasRegion">
        <rdfs:subPropertyOf rdf:resource="http://www.w3.org/2002/07/owl#topObjectProperty"/>
        <rdfs:range rdf:resource="http://www.semanticweb.org/user/ontologies/2020/CovidOntology/1.0.0#Region"/>
        <rdfs:comment>This is the region to which an entity relates.
For Country this means the country contains said region.
For a Case this means the case in which it was located.</rdfs:comment>
    </owl:ObjectProperty>
    


    <!-- 
    ///////////////////////////////////////////////////////////////////////////////////////
    //
    // Data properties
    //
    ///////////////////////////////////////////////////////////////////////////////////////
     -->

    


    <!-- http://www.semanticweb.org/user/ontologies/2020/CovidOntology/1.0.0#date -->

    <owl:DatatypeProperty rdf:about="http://www.semanticweb.org/user/ontologies/2020/CovidOntology/1.0.0#date">
        <rdfs:subPropertyOf rdf:resource="http://www.w3.org/2002/07/owl#topDataProperty"/>
        <rdfs:domain rdf:resource="http://www.semanticweb.org/user/ontologies/2020/CovidOntology/1.0.0#Day"/>
        <rdfs:range rdf:resource="http://www.w3.org/2001/XMLSchema#dateTime"/>
        <owl:propertyDisjointWith rdf:resource="http://www.semanticweb.org/user/ontologies/2020/CovidOntology/1.0.0#numberConfirmedCases"/>
        <rdfs:comment>The literal calender day.
The time in all values is 00:00:00. This is not meaningful, protege just prefers dateTime rather than simply date.</rdfs:comment>
    </owl:DatatypeProperty>
    


    <!-- http://www.semanticweb.org/user/ontologies/2020/CovidOntology/1.0.0#death -->

    <owl:DatatypeProperty rdf:about="http://www.semanticweb.org/user/ontologies/2020/CovidOntology/1.0.0#death">
        <rdfs:subPropertyOf rdf:resource="http://www.semanticweb.org/user/ontologies/2020/CovidOntology/1.0.0#numberConfirmedCases"/>
        <rdfs:comment>Number of deaths from Covid19 infection during a given region/day.</rdfs:comment>
    </owl:DatatypeProperty>
    


    <!-- http://www.semanticweb.org/user/ontologies/2020/CovidOntology/1.0.0#numberConfirmedCases -->

    <owl:DatatypeProperty rdf:about="http://www.semanticweb.org/user/ontologies/2020/CovidOntology/1.0.0#numberConfirmedCases">
        <rdfs:domain rdf:resource="http://www.semanticweb.org/user/ontologies/2020/CovidOntology/1.0.0#Case"/>
        <rdfs:range rdf:resource="http://www.w3.org/2001/XMLSchema#nonNegativeInteger"/>
        <rdfs:comment>Total number of confirmed cases.</rdfs:comment>
    </owl:DatatypeProperty>
    


    <!-- http://www.semanticweb.org/user/ontologies/2020/CovidOntology/1.0.0#recovered -->

    <owl:DatatypeProperty rdf:about="http://www.semanticweb.org/user/ontologies/2020/CovidOntology/1.0.0#recovered">
        <rdfs:subPropertyOf rdf:resource="http://www.semanticweb.org/user/ontologies/2020/CovidOntology/1.0.0#numberConfirmedCases"/>
        <rdfs:comment>Number of people who had Covid but are known to have survived in a given Region / Day.</rdfs:comment>
    </owl:DatatypeProperty>
    


    <!-- http://www.semanticweb.org/user/ontologies/2020/CovidOntology/1.0.0#unknownSurvival -->

    <owl:DatatypeProperty rdf:about="http://www.semanticweb.org/user/ontologies/2020/CovidOntology/1.0.0#unknownSurvival">
        <rdfs:subPropertyOf rdf:resource="http://www.semanticweb.org/user/ontologies/2020/CovidOntology/1.0.0#numberConfirmedCases"/>
        <rdfs:comment>Most cases, where there is a confirmed infection with Covid19 however the outcome is not well documented.</rdfs:comment>
    </owl:DatatypeProperty>
    


    <!-- 
    ///////////////////////////////////////////////////////////////////////////////////////
    //
    // Classes
    //
    ///////////////////////////////////////////////////////////////////////////////////////
     -->

    


    <!-- http://www.semanticweb.org/user/ontologies/2020/CovidOntology/1.0.0#Case -->

    <owl:Class rdf:about="http://www.semanticweb.org/user/ontologies/2020/CovidOntology/1.0.0#Case">
        <rdfs:comment>This is not an individual case of Covid19. Instead this the set of known cases during a specific day and place.</rdfs:comment>
        <rdfs:label>Covid19CaseSet</rdfs:label>
    </owl:Class>
    


    <!-- http://www.semanticweb.org/user/ontologies/2020/CovidOntology/1.0.0#Country -->

    <owl:Class rdf:about="http://www.semanticweb.org/user/ontologies/2020/CovidOntology/1.0.0#Country">
        <rdfs:subClassOf rdf:resource="http://www.semanticweb.org/user/ontologies/2020/CovidOntology/1.0.0#Location"/>
        <owl:disjointWith rdf:resource="http://www.semanticweb.org/user/ontologies/2020/CovidOntology/1.0.0#Region"/>
        <rdfs:comment>Country entities have regions with specific cases. The countries themselves do not reference the cases within themselves directly.</rdfs:comment>
    </owl:Class>
    


    <!-- http://www.semanticweb.org/user/ontologies/2020/CovidOntology/1.0.0#Day -->

    <owl:Class rdf:about="http://www.semanticweb.org/user/ontologies/2020/CovidOntology/1.0.0#Day">
        <rdfs:comment>This entity references all the cases that occured during a specific calender day.</rdfs:comment>
    </owl:Class>
    


    <!-- http://www.semanticweb.org/user/ontologies/2020/CovidOntology/1.0.0#Location -->

    <owl:Class rdf:about="http://www.semanticweb.org/user/ontologies/2020/CovidOntology/1.0.0#Location"/>
    


    <!-- http://www.semanticweb.org/user/ontologies/2020/CovidOntology/1.0.0#Region -->

    <owl:Class rdf:about="http://www.semanticweb.org/user/ontologies/2020/CovidOntology/1.0.0#Region">
        <rdfs:subClassOf rdf:resource="http://www.semanticweb.org/user/ontologies/2020/CovidOntology/1.0.0#Location"/>
        <rdfs:comment>Places within a country where case instances occured.</rdfs:comment>
    </owl:Class>
    


    <!-- 
    ///////////////////////////////////////////////////////////////////////////////////////
    //
    // Individuals
    //
    ///////////////////////////////////////////////////////////////////////////////////////
     -->

    


    <!-- http://www.semanticweb.org/user/ontologies/2020/CovidOntology/1.0.0#Australia -->

    <owl:NamedIndividual rdf:about="http://www.semanticweb.org/user/ontologies/2020/CovidOntology/1.0.0#Australia">
        <rdf:type rdf:resource="http://www.semanticweb.org/user/ontologies/2020/CovidOntology/1.0.0#Country"/>
        <hasRegion rdf:resource="http://www.semanticweb.org/user/ontologies/2020/CovidOntology/1.0.0#Syndey"/>
    </owl:NamedIndividual>
    


    <!-- http://www.semanticweb.org/user/ontologies/2020/CovidOntology/1.0.0#Case0 -->

    <owl:NamedIndividual rdf:about="http://www.semanticweb.org/user/ontologies/2020/CovidOntology/1.0.0#Case0">
        <rdf:type rdf:resource="http://www.semanticweb.org/user/ontologies/2020/CovidOntology/1.0.0#Case"/>
        <hasDay rdf:resource="http://www.semanticweb.org/user/ontologies/2020/CovidOntology/1.0.0#Day0"/>
        <hasRegion rdf:resource="http://www.semanticweb.org/user/ontologies/2020/CovidOntology/1.0.0#Syndey"/>
        <death rdf:datatype="http://www.w3.org/2001/XMLSchema#nonNegativeInteger">50</death>
        <recovered rdf:datatype="http://www.w3.org/2001/XMLSchema#nonNegativeInteger">100</recovered>
        <unknownSurvival rdf:datatype="http://www.w3.org/2001/XMLSchema#nonNegativeInteger">1000</unknownSurvival>
    </owl:NamedIndividual>
    


    <!-- http://www.semanticweb.org/user/ontologies/2020/CovidOntology/1.0.0#Case1 -->

    <owl:NamedIndividual rdf:about="http://www.semanticweb.org/user/ontologies/2020/CovidOntology/1.0.0#Case1">
        <rdf:type rdf:resource="http://www.semanticweb.org/user/ontologies/2020/CovidOntology/1.0.0#Case"/>
        <hasDay rdf:resource="http://www.semanticweb.org/user/ontologies/2020/CovidOntology/1.0.0#Day0"/>
        <hasRegion rdf:resource="http://www.semanticweb.org/user/ontologies/2020/CovidOntology/1.0.0#Syndey"/>
    </owl:NamedIndividual>
    


    <!-- http://www.semanticweb.org/user/ontologies/2020/CovidOntology/1.0.0#Day0 -->

    <owl:NamedIndividual rdf:about="http://www.semanticweb.org/user/ontologies/2020/CovidOntology/1.0.0#Day0">
        <rdf:type rdf:resource="http://www.semanticweb.org/user/ontologies/2020/CovidOntology/1.0.0#Day"/>
        <hasCase rdf:resource="http://www.semanticweb.org/user/ontologies/2020/CovidOntology/1.0.0#Case0"/>
        <hasCase rdf:resource="http://www.semanticweb.org/user/ontologies/2020/CovidOntology/1.0.0#Case1"/>
        <hasRegion rdf:resource="http://www.semanticweb.org/user/ontologies/2020/CovidOntology/1.0.0#Syndey"/>
        <date rdf:datatype="http://www.w3.org/2001/XMLSchema#dateTime">2020-03-12T00:00:00</date>
    </owl:NamedIndividual>
    


    <!-- http://www.semanticweb.org/user/ontologies/2020/CovidOntology/1.0.0#Syndey -->

    <owl:NamedIndividual rdf:about="http://www.semanticweb.org/user/ontologies/2020/CovidOntology/1.0.0#Syndey">
        <rdf:type rdf:resource="http://www.semanticweb.org/user/ontologies/2020/CovidOntology/1.0.0#Region"/>
        <hasCase rdf:resource="http://www.semanticweb.org/user/ontologies/2020/CovidOntology/1.0.0#Case0"/>
        <hasCase rdf:resource="http://www.semanticweb.org/user/ontologies/2020/CovidOntology/1.0.0#Case1"/>
        <hasCountry rdf:resource="http://www.semanticweb.org/user/ontologies/2020/CovidOntology/1.0.0#Australia"/>
    </owl:NamedIndividual>
    


    <!-- 
    ///////////////////////////////////////////////////////////////////////////////////////
    //
    // General axioms
    //
    ///////////////////////////////////////////////////////////////////////////////////////
     -->

    <rdf:Description>
        <rdf:type rdf:resource="http://www.w3.org/2002/07/owl#AllDisjointClasses"/>
        <owl:members rdf:parseType="Collection">
            <rdf:Description rdf:about="http://www.semanticweb.org/user/ontologies/2020/CovidOntology/1.0.0#Case"/>
            <rdf:Description rdf:about="http://www.semanticweb.org/user/ontologies/2020/CovidOntology/1.0.0#Day"/>
            <rdf:Description rdf:about="http://www.semanticweb.org/user/ontologies/2020/CovidOntology/1.0.0#Location"/>
        </owl:members>
    </rdf:Description>
    <rdf:Description>
        <rdf:type rdf:resource="http://www.w3.org/2002/07/owl#AllDisjointProperties"/>
        <owl:members rdf:parseType="Collection">
            <rdf:Description rdf:about="http://www.semanticweb.org/user/ontologies/2020/CovidOntology/1.0.0#hasCountry"/>
            <rdf:Description rdf:about="http://www.semanticweb.org/user/ontologies/2020/CovidOntology/1.0.0#hasDay"/>
            <rdf:Description rdf:about="http://www.semanticweb.org/user/ontologies/2020/CovidOntology/1.0.0#hasRegion"/>
        </owl:members>
    </rdf:Description>
</rdf:RDF>



<!-- Generated by the OWL API (version 4.5.9.2019-02-01T07:24:44Z) https://github.com/owlcs/owlapi -->

